upd(wip): rename Universe to UnivLvl, family to Sort and Sort to Universe

common/theories/Universes.v
@@ -1,7 +1,7 @@
 From Stdlib Require Import OrdersAlt MSetList MSetAVL MSetFacts MSetProperties MSetDecide FMapAVL.
 From Equations Require Import Equations.
 From MetaRocq.Utils Require Import utils MRMSets MRFSets.
-From MetaRocq.Common Require Import BasicAst config.
+From MetaRocq.Common Require Import BasicAst config Levels Sorts.
 From Stdlib Require Import ssreflect.
 
 Local Open Scope nat_scope.
@@ -9,1626 +9,176 @@ Local Open Scope string_scope2.
 
 Implicit Types (cf : checker_flags).
 
-Ltac absurd :=
-  match goal with
-  | [H: ~ True |- _] => elim (H I)
-  | [H : False |- _] => elim H
-  | H: is_true false |- _ => discriminate H
-  | |- False -> _ => let H := fresh in intro H; elim H
-  | |- _ -> False -> _ => let H := fresh in intros ? H; elim H
-  | |- is_true false -> _ => let H := fresh in intro H; discriminate H
-  | |- _ -> is_true false -> _ => let H := fresh in intros ? H; discriminate H
-  end.
-#[global]
-Hint Extern 10 => absurd : core.
-
-(** * Valuations *)
-
-(** A valuation is a universe level (nat) given for each
-    universe lvariable (Level.t).
-    It is >= for polymorphic concrete_sort and > 0 for monomorphic concrete_sort. *)
-Record valuation :=
-  { valuation_mono : string -> positive ;
-    valuation_poly : nat -> nat }.
-
-Class Evaluable (A : Type) := val : valuation -> A -> nat.
-
-
-(** Levels are Set or Level or lvar *)
-Module Level.
-  Inductive t_ : Set :=
-  | lzero
-  | level (_ : string)
-  | lvar (_ : nat) (* these are debruijn indices *).
-  Derive NoConfusion for t_.
-
-  Definition t := t_.
-
-  Definition is_set (x : t) :=
-    match x with
-    | lzero => true
-    | _ => false
-    end.
-
-  Definition is_var (l : t) :=
-    match l with
-    | lvar _ => true
-    | _ => false
-    end.
-
-  Global Instance Evaluable : Evaluable t
-    := fun v l => match l with
-               | lzero =>  (0%nat)
-               | level s => (Pos.to_nat (v.(valuation_mono) s))
-               | lvar x => (v.(valuation_poly) x)
-               end.
-
-
-  Definition compare (l1 l2 : t) : comparison :=
-    match l1, l2 with
-    | lzero, lzero => Eq
-    | lzero, _ => Lt
-    | _, lzero => Gt
-    | level s1, level s2 => string_compare s1 s2
-    | level _, _ => Lt
-    | _, level _ => Gt
-    | lvar n, lvar m => Nat.compare n m
-    end.
-
-  Definition eq : t -> t -> Prop := eq.
-  Definition eq_equiv : Equivalence eq := _.
-
-  Inductive lt_ : t -> t -> Prop :=
-  | ltSetLevel s : lt_ lzero (level s)
-  | ltSetlvar n : lt_ lzero (lvar n)
-  | ltLevelLevel s s' : StringOT.lt s s' -> lt_ (level s) (level s')
-  | ltLevellvar s n : lt_ (level s) (lvar n)
-  | ltlvarlvar n n' : Nat.lt n n' -> lt_ (lvar n) (lvar n').
-  Derive Signature for lt_.
-
-  Definition lt := lt_.
-
-  Definition lt_strorder : StrictOrder lt.
-  Proof.
-    constructor.
-    - intros [| |] X; inversion X.
-      now eapply irreflexivity in H1.
-      eapply Nat.lt_irrefl; tea.
-    - intros [| |] [| |] [| |] X1 X2;
-        inversion X1; inversion X2; constructor.
-      now transitivity s0.
-      etransitivity; tea.
-  Qed.
-
-  Definition lt_compat : Proper (eq ==> eq ==> iff) lt.
-  Proof.
-    intros x y e z t e'. unfold eq in *; subst. reflexivity.
-  Qed.
-
-  Definition compare_spec :
-    forall x y : t, CompareSpec (x = y) (lt x y) (lt y x) (compare x y).
-  Proof.
-    intros [] []; repeat constructor.
-    - eapply CompareSpec_Proper.
-      5: eapply CompareSpec_string. 4: reflexivity.
-      all: split; [now inversion 1|]. now intros ->.
-      all: intro; now constructor.
-    - eapply CompareSpec_Proper.
-      5: eapply Nat.compare_spec. 4: reflexivity.
-      all: split; [now inversion 1|]. now intros ->.
-      all: intro; now constructor.
-  Qed.
-
-  Definition eq_level l1 l2 :=
-    match l1, l2 with
-    | Level.lzero, Level.lzero => true
-    | Level.level     s1, Level.level     s2 => ReflectEq.eqb s1 s2
-    | Level.lvar n1, Level.lvar n2 => ReflectEq.eqb n1 n2
-    | _, _ => false
-    end.
-
-  #[global, program] Instance reflect_level : ReflectEq Level.t := {
-    eqb := eq_level
-  }.
-  Next Obligation.
-    destruct x, y.
-    all: unfold eq_level.
-    all: try solve [ constructor ; reflexivity ].
-    all: try solve [ constructor ; discriminate ].
-    - destruct (ReflectEq.eqb_spec t0 t1) ; nodec.
-      constructor. f_equal. assumption.
-    - destruct (ReflectEq.eqb_spec n n0) ; nodec.
-      constructor. subst. reflexivity.
-  Defined.
-
-  Global Instance eqb_refl : @Reflexive Level.t eqb.
-  Proof.
-    intros x. apply ReflectEq.eqb_refl.
-  Qed.
-
-  Definition eqb := eq_level.
-
-  Lemma eqb_spec l l' : reflect (eq l l') (eqb l l').
-  Proof.
-    apply reflectProp_reflect.
-    now generalize (eqb_spec l l').
-  Qed.
-
-  Definition eq_leibniz (x y : t) : eq x y -> x = y := id.
-
-  Definition eq_dec : forall (l1 l2 : t), {l1 = l2}+{l1 <> l2} := Classes.eq_dec.
-
-End Level.
-
-Module LevelSet := MSetAVL.Make Level.
-Module LevelSetFact := WFactsOn Level LevelSet.
-Module LevelSetOrdProp := MSetProperties.OrdProperties LevelSet.
-Module LevelSetProp := LevelSetOrdProp.P.
-Module LevelSetDecide := LevelSetProp.Dec.
-Module LevelSetExtraOrdProp := MSets.ExtraOrdProperties LevelSet LevelSetOrdProp.
-Module LevelSetExtraDecide := MSetAVL.Decide Level LevelSet.
-Module LS := LevelSet.
-
-Ltac lsets := LevelSetDecide.fsetdec.
-Notation "(=_lset)" := LevelSet.Equal (at level 0).
-Infix "=_lset" := LevelSet.Equal (at level 30).
-Notation "(==_lset)" := LevelSet.equal (at level 0).
-Infix "==_lset" := LevelSet.equal (at level 30).
-
-Section LevelSetMoreFacts.
-
-  Definition LevelSet_pair x y
-    := LevelSet.add y (LevelSet.singleton x).
-
-  Lemma LevelSet_pair_In x y z :
-    LevelSet.In x (LevelSet_pair y z) -> x = y \/ x = z.
-  Proof.
-    intro H. apply LevelSetFact.add_iff in H.
-    destruct H; [intuition|].
-    apply LevelSetFact.singleton_1 in H; intuition.
-  Qed.
-
-  Definition LevelSet_mem_union (s s' : LevelSet.t) x :
-    LevelSet.mem x (LevelSet.union s s') <-> LevelSet.mem x s \/ LevelSet.mem x s'.
-  Proof.
-    rewrite LevelSetFact.union_b.
-    apply orb_true_iff.
-  Qed.
-
-  Lemma LevelSet_In_fold_right_add x l :
-    In x l <-> LevelSet.In x (fold_right LevelSet.add LevelSet.empty l).
-  Proof.
-    split.
-    - induction l; simpl => //.
-      intros [<-|H].
-      * eapply LevelSet.add_spec; left; auto.
-      * eapply LevelSet.add_spec; right; auto.
-    - induction l; simpl => //.
-      * now rewrite LevelSetFact.empty_iff.
-      * rewrite LevelSet.add_spec. intuition auto.
-  Qed.
-
-  Lemma LevelSet_union_empty s : LevelSet.Equal (LevelSet.union LevelSet.empty s) s.
-  Proof.
-    intros x; rewrite LevelSet.union_spec. lsets.
-  Qed.
-End LevelSetMoreFacts.
-
-(* prop level is Prop or SProp *)
-Module PropLevel.
-
-  Inductive t := lSProp | lProp.
-  Derive NoConfusion EqDec for t.
-  (* Global Instance PropLevel_Evaluable : Evaluable t :=
-    fun v l => match l with
-              lSProp => -1
-            | lProp => -1
-            end. *)
-
-  Definition compare (l1 l2 : t) : comparison :=
-    match l1, l2 with
-    | lSProp, lSProp  => Eq
-    | lProp, lProp  => Eq
-    | lProp, lSProp => Gt
-    | lSProp, lProp => Lt
-    end.
-
-  Inductive lt_ : t -> t -> Prop :=
-    ltSPropProp : lt_ lSProp lProp.
-
-  Definition lt := lt_.
-
-  Global Instance lt_strorder : StrictOrder lt.
-  split.
-  - intros n X. destruct n;inversion X.
-  - intros n1 n2 n3 X1 X2. destruct n1,n2,n3;auto; try inversion X1;try inversion X2.
-  Defined.
-
-End PropLevel.
-
-Module LevelExpr.
-  Definition t := (Level.t * nat)%type.
-
-  Global Instance Evaluable : Evaluable t
-    := fun v l => (snd l + val v (fst l)).
-
-  Definition succ (l : t) := (fst l, S (snd l)).
-
-  Definition get_level (e : t) : Level.t := fst e.
-
-  Definition get_noprop (e : LevelExpr.t) := Some (fst e).
-
-  Definition is_level (e : t) : bool :=
-    match e with
-    | (_, 0%nat) => true
-    | _  => false
-    end.
-
-  Definition make (l : Level.t) : t := (l, 0%nat).
-
-  Definition set : t := (Level.lzero, 0%nat).
-  Definition type1 : t := (Level.lzero, 1%nat).
-
-  Definition eq : t -> t -> Prop := eq.
-
-  Definition eq_equiv : Equivalence eq := _.
-
-  Inductive lt_ : t -> t -> Prop :=
-  | ltLevelExpr1 l n n' : (n < n')%nat -> lt_ (l, n) (l, n')
-  | ltLevelExpr2 l l' b b' : Level.lt l l' -> lt_ (l, b) (l', b').
-
-  Definition lt := lt_.
-
-  Global Instance lt_strorder : StrictOrder lt.
-  Proof.
-    constructor.
-    - intros x X; inversion X. subst. lia. subst.
-      eapply Level.lt_strorder; eassumption.
-    - intros x y z X1 X2; invs X1; invs X2; constructor; tea.
-      etransitivity; tea.
-      etransitivity; tea.
-  Qed.
-
-  Definition lt_compat : Proper (Logic.eq ==> Logic.eq ==> iff) lt.
-    intros x x' H1 y y' H2; now rewrite H1 H2.
-  Qed.
-
-  Definition compare (x y : t) : comparison :=
-    match x, y with
-    | (l1, b1), (l2, b2) =>
-      match Level.compare l1 l2 with
-      | Eq => Nat.compare b1 b2
-      | x => x
-      end
-    end.
-
-  Definition compare_spec :
-    forall x y : t, CompareSpec (x = y) (lt x y) (lt y x) (compare x y).
-  Proof.
-    intros [? ?] [? ?]; cbn; repeat constructor.
-    destruct (Level.compare_spec t0 t1); repeat constructor; tas.
-    subst.
-    destruct (Nat.compare_spec n n0); repeat constructor; tas. congruence.
-  Qed.
-
-  Global Instance reflect_t : ReflectEq t := reflect_prod _ _ .
-
-  Definition eq_dec : forall (l1 l2 : t), {l1 = l2} + {l1 <> l2} := Classes.eq_dec.
-
-  Definition eq_leibniz (x y : t) : eq x y -> x = y := id.
-
-  Lemma val_make v l
-    : val v (LevelExpr.make l) = val v l.
-  Proof.
-    destruct l eqn:H; cbnr.
-  Qed.
-
-  Lemma val_make_npl v (l : Level.t)
-    : val v (LevelExpr.make l) = val v l.
-  Proof.
-    destruct l; cbnr.
-  Qed.
-
-End LevelExpr.
-
-Module LevelExprSet := MSetList.MakeWithLeibniz LevelExpr.
-Module LevelExprSetFact := WFactsOn LevelExpr LevelExprSet.
-Module LevelExprSetOrdProp := MSetProperties.OrdProperties LevelExprSet.
-Module LevelExprSetProp := LevelExprSetOrdProp.P.
-Module LevelExprSetDecide := LevelExprSetProp.Dec.
-Module LevelExprSetExtraOrdProp := MSets.ExtraOrdProperties LevelExprSet LevelExprSetOrdProp.
-
-(* We have decidable equality w.r.t leibniz equality for sets of levels.
-  This means concrete_sort also has a decidable equality. *)
-#[global, program] Instance levelexprset_reflect : ReflectEq LevelExprSet.t :=
-  { eqb := LevelExprSet.equal }.
-Next Obligation.
-  destruct (LevelExprSet.equal x y) eqn:e; constructor.
-  eapply LevelExprSet.equal_spec in e.
-  now eapply LevelExprSet.eq_leibniz.
-  intros e'.
-  subst y.
-  pose proof (@LevelExprSetFact.equal_1 x x).
-  forward H. reflexivity. congruence.
-Qed.
-
-#[global] Instance levelexprset_eq_dec : Classes.EqDec LevelExprSet.t := Classes.eq_dec.
-
-
-
-Record nonEmptyLevelExprSet
-  := { t_set : LevelExprSet.t ;
-       t_ne  : LevelExprSet.is_empty t_set = false }.
-
-Derive NoConfusion for nonEmptyLevelExprSet.
-
-(** This coercion allows to see the non-empty set as a regular [LevelExprSet.t] *)
-Coercion t_set : nonEmptyLevelExprSet >-> LevelExprSet.t.
-
-Module NonEmptySetFacts.
-  Definition singleton (e : LevelExpr.t) : nonEmptyLevelExprSet
-    := {| t_set := LevelExprSet.singleton e;
-          t_ne := eq_refl |}.
-
-  Lemma not_Empty_is_empty s :
-    ~ LevelExprSet.Empty s -> LevelExprSet.is_empty s = false.
-  Proof.
-    intro H. apply not_true_is_false. intro H'.
-    apply H. now apply LevelExprSetFact.is_empty_2 in H'.
-  Qed.
-
-  Program Definition add (e : LevelExpr.t) (u : nonEmptyLevelExprSet) : nonEmptyLevelExprSet
-    := {| t_set := LevelExprSet.add e u |}.
-  Next Obligation.
-    apply not_Empty_is_empty; intro H.
-    eapply H. eapply LevelExprSet.add_spec.
-    left; reflexivity.
-  Qed.
-
-  Lemma add_spec e u e' :
-    LevelExprSet.In e' (add e u) <-> e' = e \/ LevelExprSet.In e' u.
-  Proof.
-    apply LevelExprSet.add_spec.
-  Qed.
-
-  Definition add_list : list LevelExpr.t -> nonEmptyLevelExprSet -> nonEmptyLevelExprSet
-    := List.fold_left (fun u e => add e u).
-
-  Lemma add_list_spec l u e :
-    LevelExprSet.In e (add_list l u) <-> In e l \/ LevelExprSet.In e u.
-  Proof.
-    unfold add_list. rewrite <- fold_left_rev_right.
-    etransitivity. 2:{ eapply or_iff_compat_r. etransitivity.
-                       2: apply @InA_In_eq with (A:=LevelExpr.t).
-                       eapply InA_rev. }
-    induction (List.rev l); cbn.
-    - split. intuition. intros [H|H]; tas. invs H.
-    - split.
-      + intro H. apply add_spec in H. destruct H as [H|H].
-        * left. now constructor.
-        * apply IHl0 in H. destruct H as [H|H]; [left|now right].
-          now constructor 2.
-      + intros [H|H]. inv H.
-        * apply add_spec; now left.
-        * apply add_spec; right. apply IHl0. now left.
-        * apply add_spec; right. apply IHl0. now right.
-  Qed.
-
-  Program Definition to_nonempty_list (u : nonEmptyLevelExprSet) : LevelExpr.t * list LevelExpr.t
-    := match LevelExprSet.elements u with
-       | [] => False_rect _ _
-       | e :: l => (e, l)
-       end.
-  Next Obligation.
-    destruct u as [u1 u2]; cbn in *. revert u2.
-    apply eq_true_false_abs.
-    unfold LevelExprSet.is_empty, LevelExprSet.Raw.is_empty,
-    LevelExprSet.elements, LevelExprSet.Raw.elements in *.
-    rewrite <- Heq_anonymous; reflexivity.
-  Qed.
-
-  Lemma singleton_to_nonempty_list e : to_nonempty_list (singleton e) = (e, []).
-  Proof. reflexivity. Defined.
-
-  Lemma to_nonempty_list_spec u :
-    let '(e, u') := to_nonempty_list u in
-    e :: u' = LevelExprSet.elements u.
-  Proof.
-    destruct u as [u1 u2].
-    unfold to_nonempty_list; cbn.
-    set (l := LevelExprSet.elements u1). unfold l at 2 3 4.
-    set (e := (eq_refl: l = LevelExprSet.elements u1)); clearbody e.
-    destruct l.
-    - exfalso. revert u2. apply eq_true_false_abs.
-      unfold LevelExprSet.is_empty, LevelExprSet.Raw.is_empty,
-      LevelExprSet.elements, LevelExprSet.Raw.elements in *.
-      rewrite <- e; reflexivity.
-    - reflexivity.
-  Qed.
-
-  Lemma to_nonempty_list_spec' u :
-    (to_nonempty_list u).1 :: (to_nonempty_list u).2 = LevelExprSet.elements u.
-  Proof.
-    pose proof (to_nonempty_list_spec u).
-    now destruct (to_nonempty_list u).
-  Qed.
-
-  Lemma In_to_nonempty_list (u : nonEmptyLevelExprSet) (e : LevelExpr.t) :
-    LevelExprSet.In e u
-    <-> e = (to_nonempty_list u).1 \/ In e (to_nonempty_list u).2.
-  Proof.
-    etransitivity. symmetry. apply LevelExprSet.elements_spec1.
-    pose proof (to_nonempty_list_spec' u) as H.
-    destruct (to_nonempty_list u) as [e' l]; cbn in *.
-    rewrite <- H; clear. etransitivity. apply InA_cons.
-    eapply or_iff_compat_l. apply InA_In_eq.
-  Qed.
-
-  Lemma In_to_nonempty_list_rev (u : nonEmptyLevelExprSet) (e : LevelExpr.t) :
-    LevelExprSet.In e u
-    <-> e = (to_nonempty_list u).1 \/ In e (List.rev (to_nonempty_list u).2).
-  Proof.
-    etransitivity. eapply In_to_nonempty_list.
-    apply or_iff_compat_l. apply in_rev.
-  Qed.
-
-  Definition map (f : LevelExpr.t -> LevelExpr.t) (u : nonEmptyLevelExprSet) : nonEmptyLevelExprSet :=
-    let '(e, l) := to_nonempty_list u in
-    add_list (List.map f l) (singleton (f e)).
-
-  Lemma map_spec f u e :
-    LevelExprSet.In e (map f u) <-> exists e0, LevelExprSet.In e0 u /\ e = (f e0).
-  Proof.
-    unfold map. symmetry. etransitivity.
-    { eapply iff_ex; intro. eapply and_iff_compat_r. eapply In_to_nonempty_list. }
-    destruct (to_nonempty_list u) as [e' l]; cbn in *.
-    symmetry. etransitivity. eapply add_list_spec.
-    etransitivity. eapply or_iff_compat_l. apply LevelExprSet.singleton_spec.
-    etransitivity. eapply or_iff_compat_r.
-    apply in_map_iff. clear u. split.
-    - intros [[e0 []]|H].
-      + exists e0. split. right; tas. congruence.
-      + exists e'. split; tas. left; reflexivity.
-    - intros [xx [[H|H] ?]].
-      + right. congruence.
-      + left. exists xx. split; tas; congruence.
-  Qed.
-
-  Program Definition non_empty_union (u v : nonEmptyLevelExprSet) : nonEmptyLevelExprSet :=
-    {| t_set := LevelExprSet.union u v |}.
-  Next Obligation.
-    apply not_Empty_is_empty; intro H.
-    assert (HH: LevelExprSet.Empty u). {
-      intros x Hx. apply (H x).
-      eapply LevelExprSet.union_spec. now left. }
-    apply LevelExprSetFact.is_empty_1 in HH.
-    rewrite t_ne in HH; discriminate.
-  Qed.
-
-  Lemma elements_not_empty (u : nonEmptyLevelExprSet) : LevelExprSet.elements u <> [].
-  Proof.
-    destruct u as [u1 u2]; cbn; intro e.
-    unfold LevelExprSet.is_empty, LevelExprSet.elements,
-    LevelExprSet.Raw.elements in *.
-    rewrite e in u2; discriminate.
-  Qed.
-
-
-  Lemma eq_univ (u v : nonEmptyLevelExprSet) :
-    u = v :> LevelExprSet.t -> u = v.
-  Proof.
-    destruct u as [u1 u2], v as [v1 v2]; cbn. intros X; destruct X.
-    now rewrite (uip_bool _ _ u2 v2).
-  Qed.
-
-  Lemma eq_univ' (u v : nonEmptyLevelExprSet) :
-    LevelExprSet.Equal u v -> u = v.
-  Proof.
-    intro H. now apply eq_univ, LevelExprSet.eq_leibniz.
-  Qed.
-
-  Lemma eq_univ'' (u v : nonEmptyLevelExprSet) :
-    LevelExprSet.elements u = LevelExprSet.elements v -> u = v.
-  Proof.
-    intro H. apply eq_univ.
-    destruct u as [u1 u2], v as [v1 v2]; cbn in *; clear u2 v2.
-    destruct u1 as [u1 u2], v1 as [v1 v2]; cbn in *.
-    destruct H. now rewrite (uip_bool _ _ u2 v2).
-  Qed.
-
-  Lemma univ_expr_eqb_true_iff (u v : nonEmptyLevelExprSet) :
-    LevelExprSet.equal u v <-> u = v.
-  Proof.
-    split.
-    - intros.
-      apply eq_univ'. now apply LevelExprSet.equal_spec.
-    - intros ->. now apply LevelExprSet.equal_spec.
-  Qed.
-
-  Lemma univ_expr_eqb_comm (u v : nonEmptyLevelExprSet) :
-    LevelExprSet.equal u v <-> LevelExprSet.equal v u.
-  Proof.
-    transitivity (u = v). 2: transitivity (v = u).
-    - apply univ_expr_eqb_true_iff.
-    - split; apply eq_sym.
-    - split; apply univ_expr_eqb_true_iff.
-  Qed.
-
-
-  Lemma LevelExprSet_for_all_false f u :
-    LevelExprSet.for_all f u = false -> LevelExprSet.exists_ (negb ∘ f) u.
-  Proof.
-    intro H. rewrite LevelExprSetFact.exists_b.
-    rewrite LevelExprSetFact.for_all_b in H.
-    all: try now intros x y [].
-    induction (LevelExprSet.elements u); cbn in *; [discriminate|].
-    apply andb_false_iff in H; apply orb_true_iff; destruct H as [H|H].
-    left; now rewrite H.
-    right; now rewrite IHl.
-  Qed.
-
-  Lemma LevelExprSet_For_all_exprs (P : LevelExpr.t -> Prop) (u : nonEmptyLevelExprSet)
-    : LevelExprSet.For_all P u
-      <-> P (to_nonempty_list u).1 /\ Forall P (to_nonempty_list u).2.
-  Proof.
-    etransitivity.
-    - eapply iff_forall; intro e. eapply imp_iff_compat_r.
-      apply In_to_nonempty_list.
-    - cbn; split.
-      + intro H. split. apply H. now left.
-        apply Forall_forall. intros x H0.  apply H; now right.
-      + intros [H1 H2] e [He|He]. subst e; tas.
-        eapply Forall_forall in H2; tea.
-  Qed.
-
-
-End NonEmptySetFacts.
-Import NonEmptySetFacts.
-
-
 Module Universe.
-  (** A universe / an algebraic expression is a list of universe expressions which is:
-        - sorted
-        - without duplicate
-        - non empty *)
+  (** A Universe is a product of a sort with a universe level.
 
-  Definition t := nonEmptyLevelExprSet.
+  	  Universes are quotiented at conversion so that every impredicative sorts (e.g., [sSProp] or [sProp])
+	  at level i and j are convertible. *)
+  Record t_ {sort} {ulvl} :=
+    mkUniv
+	{ s : sort
+  	; l : ulvl }.
+  Arguments t_ : clear implicits.
+  Arguments mkUniv {_ _} _ _.
 
-  (* We use uip on the is_empty condition *)
-  #[global, program] Instance levelexprset_reflect : ReflectEq t :=
-    { eqb x y := eqb x.(t_set) y.(t_set) }.
+  Definition t := t_ Sort.t UnivLvl.t.
+
+  Definition eqb {sort} {univ} `{ReflectEq sort} `{ReflectEq univ} (u1 u2 : t_ sort univ) : bool :=
+    eqb u1.(s) u2.(s) &&
+	eqb u1.(l) u2.(l).
+
+  #[global, program] Instance reflect_eq_univ {sort} {ulvl} `{ReflectEq sort} `{ReflectEq ulvl} : ReflectEq (t_ sort ulvl) :=
+    { eqb := eqb }.
   Next Obligation.
-    destruct (eqb_spec (t_set x) (t_set y)); constructor.
-    destruct x, y; cbn in *. subst.
-    now rewrite (uip t_ne0 t_ne1).
-    intros e; subst x; apply H.
-    reflexivity.
+    destruct x as [s l], y as [s' l']; unfold eqb; cbn.
+	destruct (eqb_spec s s'); destruct (eqb_spec l l').
+	all: cbn; constructor; easy.
   Qed.
 
-  #[global] Instance eq_dec_univ0 : EqDec t := eq_dec.
+  #[global] Instance eq_dec_univ {sort} {ulvl} `{EqDec sort} `{EqDec ulvl} : EqDec (t_ sort ulvl) :=
+    ltac:(intros s s'; decide equality).
 
-  Definition make (e: LevelExpr.t) : t := singleton e.
-  Definition make' (l: Level.t) : t := singleton (LevelExpr.make l).
+  Definition map {sort sort'} {ulvl ulvl'} (fs : sort -> sort') (fl : ulvl -> ulvl') u :=
+    mkUniv (fs u.(s)) (fl u.(l)).
 
-  Lemma make'_inj l l' : make' l = make' l' -> l = l'.
-  Proof.
-    destruct l, l' => //=; now inversion 1.
-  Qed.
+  Definition maps {sort sort'} {ulvl} (f : sort -> sort') u :=
+    map f (fun (x : ulvl) => x) u.
 
-  (** The non empty / sorted / without dup list of univ expressions, the
-    components of the pair are the head and the tail of the (non empty) list *)
-  Definition exprs : t -> LevelExpr.t * list LevelExpr.t := to_nonempty_list.
+  Definition mapl {sort} {ulvl ulvl'} (f : ulvl -> ulvl') u :=
+    map (fun (x : sort) => x) f u.
 
-  Global Instance Evaluable : Evaluable Universe.t
-    := fun v u =>
-      let '(e, u) := Universe.exprs u in
-      List.fold_left (fun n e => Nat.max (val v e) n) u (val v e).
+  Definition on_sort {ulvl} {T} (P: ulvl -> T) (def: T) (u : t_ Sort.t ulvl) :=
+    match u.(s) with
+    | sProp | sSProp => def
+    | sType => P u.(l)
+    end.
 
   (** Test if the universe is a lub of levels or contains +n's. *)
   Definition is_levels (u : t) : bool :=
-    LevelExprSet.for_all LevelExpr.is_level u.
+    match u.(s) with
+    | sSProp | sProp => true
+    | sType => UnivLvl.is_levels u.(l)
+    end.
 
   (** Test if the universe is a level or an algebraic universe. *)
   Definition is_level (u : t) : bool :=
-    (LevelExprSet.cardinal u =? 1)%nat && is_levels u.
-
-  (* Used for quoting. *)
-  Definition from_kernel_repr (e : Level.t * nat) (es : list (Level.t * nat)) : t
-    := add_list es (Universe.make e).
-
-  Definition succ : t -> t := map LevelExpr.succ.
-
-  (** The l.u.b. of 2 non-prop universe sets *)
-  Definition sup : t -> t -> t := non_empty_union.
-
-  Definition get_is_level (u : t) : option Level.t :=
-    match LevelExprSet.elements u with
-    | [(l, 0%nat)] => Some l
-    | _ => None
-    end.
-
-  Lemma val_make v e : val v (make e) = val v e.
-  Proof. reflexivity. Qed.
-
-  Lemma val_make' v l
-    : val v (make' l) = val v l.
-  Proof. reflexivity. Qed.
-
-  Definition lt : t -> t -> Prop := LevelExprSet.lt.
-  Definition lt_compat : Proper (eq ==> eq ==> iff) lt.
-  Proof. repeat intro; subst; reflexivity. Qed.
-  #[global] Instance lt_strorder : StrictOrder lt.
-  Proof.
-    cbv [lt]; constructor.
-    { intros ? H. apply irreflexivity in H; assumption. }
-    { intros ??? H1 H2; etransitivity; tea. }
-  Qed.
-End Universe.
-
-Ltac u :=
-  change LevelSet.elt with Level.t in *;
-  change LevelExprSet.elt with LevelExpr.t in *.
-  (* change ConstraintSet.elt with UnivConstraint.t in *. *)
-
-
-Lemma val_fold_right (u : Universe.t) v :
-  val v u = fold_right (fun e x => Nat.max (val v e) x) (val v (Universe.exprs u).1)
-                       (List.rev (Universe.exprs u).2).
-Proof.
-  unfold val at 1, Universe.Evaluable.
-  destruct (Universe.exprs u).
-  now rewrite fold_left_rev_right.
-Qed.
-
-Lemma val_In_le (u : Universe.t) v e :
-  LevelExprSet.In e u -> val v e <= val v u.
-Proof.
-  intro H. rewrite val_fold_right.
-  apply In_to_nonempty_list_rev in H.
-  fold Universe.exprs in H; destruct (Universe.exprs u); cbn in *.
-  destruct H as [H|H].
-  - subst. induction (List.rev l); cbnr. lia.
-  - induction (List.rev l); cbn; invs H.
-    + u; lia.
-    + specialize (IHl0 H0). lia.
-Qed.
-
-Lemma val_In_max (u : Universe.t) v :
-  exists e, LevelExprSet.In e u /\ val v e = val v u.
-Proof.
-  eapply iff_ex. {
-    intro. eapply and_iff_compat_r. apply In_to_nonempty_list_rev. }
-  rewrite val_fold_right. fold Universe.exprs; destruct (Universe.exprs u) as [e l]; cbn in *.
-  clear. induction (List.rev l); cbn.
-  - exists e. split; cbnr. left; reflexivity.
-  - destruct IHl0 as [e' [H1 H2]].
-    destruct (Nat.max_dec (val v a) (fold_right (fun e0 x0 => Nat.max (val v e0) x0)
-                                               (val v e) l0)) as [H|H];
-      rewrite H; clear H.
-    + exists a. split; cbnr. right. now constructor.
-    + rewrite <- H2. exists e'. split; cbnr.
-      destruct H1 as [H1|H1]; [now left|right]. now constructor 2.
-Qed.
-
-Lemma val_ge_caract (u : Universe.t) v k :
-  (forall e, LevelExprSet.In e u -> val v e <= k) <-> val v u <= k.
-Proof.
-  split.
-  - eapply imp_iff_compat_r. {
-      eapply iff_forall; intro. eapply imp_iff_compat_r.
-      apply In_to_nonempty_list_rev. }
-    rewrite val_fold_right.
-    fold Universe.exprs; destruct (Universe.exprs u) as [e l]; cbn; clear.
-    induction (List.rev l); cbn.
-    + intros H. apply H. left; reflexivity.
-    + intros H.
-      destruct (Nat.max_dec (val v a) (fold_right (fun e0 x => Nat.max (val v e0) x)
-                                                 (val v e) l0)) as [H'|H'];
-        rewrite H'; clear H'.
-      * apply H. right. now constructor.
-      * apply IHl0. intros x [H0|H0]; apply H. now left.
-        right; now constructor 2.
-  - intros H e He. eapply val_In_le in He. etransitivity; eassumption.
-Qed.
-
-Lemma val_le_caract (u : Universe.t) v k :
-  (exists e, LevelExprSet.In e u /\ k <= val v e) <-> k <= val v u.
-Proof.
-  split.
-  - eapply imp_iff_compat_r. {
-      eapply iff_ex; intro. eapply and_iff_compat_r. apply In_to_nonempty_list_rev. }
-    rewrite val_fold_right.
-    fold Universe.exprs; destruct (Universe.exprs u) as [e l]; cbn; clear.
-    induction (List.rev l); cbn.
-    + intros H. destruct H as [e' [[H1|H1] H2]].
-      * now subst.
-      * invs H1.
-    + intros [e' [[H1|H1] H2]].
-      * forward IHl0; [|lia]. exists e'. split; tas. left; assumption.
-      * invs H1.
-        -- u; lia.
-        -- forward IHl0; [|lia]. exists e'. split; tas. right; assumption.
-  - intros H. destruct (val_In_max u v) as [e [H1 H2]].
-    exists e. rewrite H2; split; assumption.
-Qed.
-
-
-
-Lemma val_caract (u : Universe.t) v k :
-  val v u = k
-  <-> (forall e, LevelExprSet.In e u -> val v e <= k)
-    /\ exists e, LevelExprSet.In e u /\ val v e = k.
-Proof.
-  split.
-  - intros <-; split.
-    + apply val_In_le.
-    + apply val_In_max.
-  - intros [H1 H2].
-    apply val_ge_caract in H1.
-    assert (k <= val v u); [clear H1|lia].
-    apply val_le_caract. destruct H2 as [e [H2 H2']].
-    exists e. split; tas. lia.
-Qed.
-
-Lemma val_add v e (s: Universe.t)
-  : val v (add e s) = Nat.max (val v e) (val v s).
-Proof.
-  apply val_caract. split.
-  - intros e' H. apply LevelExprSet.add_spec in H. destruct H as [H|H].
-    + subst. u; lia.
-    + eapply val_In_le with (v:=v) in H. lia.
-  - destruct (Nat.max_dec (val v e) (val v s)) as [H|H]; rewrite H; clear H.
-    + exists e. split; cbnr. apply LevelExprSetFact.add_1. reflexivity.
-    + destruct (val_In_max s v) as [e' [H1 H2]].
-      exists e'. split; tas. now apply LevelExprSetFact.add_2.
-Qed.
-
-Lemma val_sup v s1 s2 :
-  val v (Universe.sup s1 s2) = Nat.max (val v s1) (val v s2).
-Proof.
-  eapply val_caract. cbn. split.
-  - intros e' H. eapply LevelExprSet.union_spec in H. destruct H as [H|H].
-    + eapply val_In_le with (v:=v) in H. lia.
-    + eapply val_In_le with (v:=v) in H. lia.
-  - destruct (Nat.max_dec (val v s1) (val v s2)) as [H|H]; rewrite H; clear H.
-    + destruct (val_In_max s1 v) as [e' [H1 H2]].
-      exists e'. split; tas. apply LevelExprSet.union_spec. now left.
-    + destruct (val_In_max s2 v) as [e' [H1 H2]].
-      exists e'. split; tas. apply LevelExprSet.union_spec. now right.
-Qed.
-
-Ltac proper := let H := fresh in try (intros ? ? H; destruct H; reflexivity).
-
-Lemma for_all_elements (P : LevelExpr.t -> bool) u :
-  LevelExprSet.for_all P u = forallb P (LevelExprSet.elements u).
-Proof.
-  apply LevelExprSetFact.for_all_b; proper.
-Qed.
-
-
-Lemma universe_get_is_level_correct u l :
-  Universe.get_is_level u = Some l -> u = Universe.make' l.
-Proof.
-  intro H.
-  unfold Universe.get_is_level in *.
-  destruct (LevelExprSet.elements u) as [|l0 L] eqn:Hu1; [discriminate |].
-  destruct l0, L; try discriminate.
-  * destruct n; inversion H; subst.
-    apply eq_univ''; apply Hu1.
-  * destruct n; discriminate.
-Qed.
-
-
-Lemma sup0_comm x1 x2 :
-  Universe.sup x1 x2 = Universe.sup x2 x1.
-Proof.
-  apply eq_univ'; simpl. unfold LevelExprSet.Equal.
-  intros H. rewrite !LevelExprSet.union_spec. intuition.
-Qed.
-
-(*
-Lemma val_zero_exprs v (l : Universe.t) : 0 <= val v l.
-Proof.
-  rewrite val_fold_right.
-  destruct (Universe.exprs l) as [e u']; clear l; cbn.
-  induction (List.rev u'); simpl.
-  - destruct e as [npl_expr].
-    destruct npl_expr as [t b].
-    cbn.
-    assert (0 <= val v t) by apply Level.val_zero.
-    destruct b;lia.
-  - pose proof (LevelExpr.val_zero a v); lia.
-Qed. *)
-
-
-Module ConstraintType.
-  Inductive t_ : Set := Le (z : Z) | Eq.
-  Derive NoConfusion EqDec for t_.
-
-  Definition t := t_.
-  Definition eq : t -> t -> Prop := eq.
-  Definition eq_equiv : Equivalence eq := _.
-
-  Definition Le0 := Le 0.
-  Definition Lt := Le 1.
-
-  Inductive lt_ : t -> t -> Prop :=
-  | LeLe n m : (n < m)%Z -> lt_ (Le n) (Le m)
-  | LeEq n : lt_ (Le n) Eq.
-  Derive Signature for lt_.
-  Definition lt := lt_.
-
-  Global Instance lt_strorder : StrictOrder lt.
-  Proof.
-    constructor.
-    - intros []; intro X; inversion X. lia.
-    - intros ? ? ? X Y; invs X; invs Y; constructor. lia.
-  Qed.
-
-  Global Instance lt_compat : Proper (eq ==> eq ==> iff) lt.
-  Proof.
-    intros ? ? X ? ? Y; invs X; invs Y. reflexivity.
-  Qed.
-
-  Definition compare (x y : t) : comparison :=
-    match x, y with
-    | Le n, Le m => Z.compare n m
-    | Le _, Eq => Datatypes.Lt
-    | Eq, Eq => Datatypes.Eq
-    | Eq, _  => Datatypes.Gt
-    end.
-
-  Lemma compare_spec x y : CompareSpec (eq x y) (lt x y) (lt y x) (compare x y).
-  Proof.
-    destruct x, y; repeat constructor. simpl.
-    destruct (Z.compare_spec z z0); simpl; constructor.
-    subst; constructor. now constructor. now constructor.
-  Qed.
-
-  Lemma eq_dec x y : {eq x y} + {~ eq x y}.
-  Proof.
-    unfold eq. decide equality. apply Z.eq_dec.
-  Qed.
-End ConstraintType.
-
-Module UnivConstraint.
-  Definition t : Set := Level.t * ConstraintType.t * Level.t.
-
-  Definition eq : t -> t -> Prop := eq.
-  Definition eq_equiv : Equivalence eq := _.
-
-  Definition make l1 ct l2 : t := (l1, ct, l2).
-
-  Inductive lt_ : t -> t -> Prop :=
-  | lt_Level2 l1 t l2 l2' : Level.lt l2 l2' -> lt_ (l1, t, l2) (l1, t, l2')
-  | lt_Cstr l1 t t' l2 l2' : ConstraintType.lt t t' -> lt_ (l1, t, l2) (l1, t', l2')
-  | lt_Level1 l1 l1' t t' l2 l2' : Level.lt l1 l1' -> lt_ (l1, t, l2) (l1', t', l2').
-  Definition lt := lt_.
-
-  Lemma lt_strorder : StrictOrder lt.
-  Proof.
-    constructor.
-    - intros []; intro X; inversion X; subst;
-        try (eapply Level.lt_strorder; eassumption).
-      eapply ConstraintType.lt_strorder; eassumption.
-    - intros ? ? ? X Y; invs X; invs Y; constructor; tea.
-      etransitivity; eassumption.
-      2: etransitivity; eassumption.
-      eapply ConstraintType.lt_strorder; eassumption.
-  Qed.
-
-  Lemma lt_compat : Proper (eq ==> eq ==> iff) lt.
-  Proof.
-    intros ? ? X ? ? Y; invs X; invs Y. reflexivity.
-  Qed.
-
-  Definition compare : t -> t -> comparison :=
-    fun '(l1, t, l2) '(l1', t', l2') =>
-      compare_cont (Level.compare l1 l1')
-        (compare_cont (ConstraintType.compare t t')
-                    (Level.compare l2 l2')).
-
-  Lemma compare_spec x y
-    : CompareSpec (eq x y) (lt x y) (lt y x) (compare x y).
-  Proof.
-    destruct x as [[l1 t] l2], y as [[l1' t'] l2']; cbn.
-    destruct (Level.compare_spec l1 l1'); cbn; repeat constructor; tas.
-    invs H.
-    destruct (ConstraintType.compare_spec t t'); cbn; repeat constructor; tas.
-    invs H.
-    destruct (Level.compare_spec l2 l2'); cbn; repeat constructor; tas.
-    invs H. reflexivity.
-  Qed.
-
-  Lemma eq_dec x y : {eq x y} + {~ eq x y}.
-  Proof.
-    unfold eq. decide equality; apply eq_dec.
-  Defined.
-
-  Definition eq_leibniz (x y : t) : eq x y -> x = y := id.
-End UnivConstraint.
-
-Module ConstraintSet := MSetAVL.Make UnivConstraint.
-Module ConstraintSetFact := WFactsOn UnivConstraint ConstraintSet.
-Module ConstraintSetOrdProp := MSetProperties.OrdProperties ConstraintSet.
-Module ConstraintSetProp := ConstraintSetOrdProp.P.
-Module CS := ConstraintSet.
-Module ConstraintSetDecide := ConstraintSetProp.Dec.
-Module ConstraintSetExtraOrdProp := MSets.ExtraOrdProperties ConstraintSet ConstraintSetOrdProp.
-Module ConstraintSetExtraDecide := MSetAVL.Decide UnivConstraint ConstraintSet.
-Ltac csets := ConstraintSetDecide.fsetdec.
-
-Notation "(=_cset)" := ConstraintSet.Equal (at level 0).
-Infix "=_cset" := ConstraintSet.Equal (at level 30).
-Notation "(==_cset)" := ConstraintSet.equal (at level 0).
-Infix "==_cset" := ConstraintSet.equal (at level 30).
-
-Definition declared_cstr_levels levels (cstr : UnivConstraint.t) :=
-  let '(l1,_,l2) := cstr in
-  LevelSet.In l1 levels /\ LevelSet.In l2 levels.
-
-Definition is_declared_cstr_levels levels (cstr : UnivConstraint.t) : bool :=
-  let '(l1,_,l2) := cstr in
-  LevelSet.mem l1 levels && LevelSet.mem l2 levels.
-
-Lemma CS_union_empty s : ConstraintSet.union ConstraintSet.empty s =_cset s.
-Proof.
-  intros x; rewrite ConstraintSet.union_spec. lsets.
-Qed.
-
-Lemma CS_For_all_union f cst cst' : ConstraintSet.For_all f (ConstraintSet.union cst cst') ->
-  ConstraintSet.For_all f cst.
-Proof.
-  unfold CS.For_all.
-  intros IH x inx. apply (IH x).
-  now eapply CS.union_spec; left.
-Qed.
-
-Lemma CS_For_all_add P x s : CS.For_all P (CS.add x s) -> P x /\ CS.For_all P s.
-Proof.
-  intros.
-  split.
-  * apply (H x), CS.add_spec; left => //.
-  * intros y iny. apply (H y), CS.add_spec; right => //.
-Qed.
-
-#[global] Instance CS_For_all_proper P : Morphisms.Proper ((=_cset) ==> iff)%signature (ConstraintSet.For_all P).
-Proof.
-  intros s s' eqs.
-  unfold CS.For_all. split; intros IH x inxs; apply (IH x);
-  now apply eqs.
-Qed.
-
-(** {6 Sort instances} *)
-
-Module Instance.
-
-  (** A universe instance represents a vector of argument concrete_sort
-      to a polymorphic definition (constant, inductive or constructor). *)
-  Definition t : Set := list Level.t.
-
-  Definition empty : t := [].
-  Definition is_empty (i : t) : bool :=
-    match i with
-    | [] => true
-    | _ => false
-    end.
-
-  Definition eqb (i j : t) :=
-    forallb2 Level.eqb i j.
-
-  Definition equal_upto (f : Level.t -> Level.t -> bool) (i j : t) :=
-    forallb2 f i j.
-End Instance.
-
-Module UContext.
-  Definition t := list name × (Instance.t × ConstraintSet.t).
-
-  Definition make' : Instance.t -> ConstraintSet.t -> Instance.t × ConstraintSet.t := pair.
-  Definition make (ids : list name) (inst_ctrs : Instance.t × ConstraintSet.t) : t := (ids, inst_ctrs).
-
-  Definition empty : t := ([], (Instance.empty, ConstraintSet.empty)).
-
-  Definition instance : t -> Instance.t := fun x => fst (snd x).
-  Definition constraints : t -> ConstraintSet.t := fun x => snd (snd x).
-
-  Definition dest : t -> list name * (Instance.t * ConstraintSet.t) := fun x => x.
-End UContext.
-
-Module AUContext.
-  Definition t := list name × ConstraintSet.t.
-
-  Definition make (ids : list name) (ctrs : ConstraintSet.t) : t := (ids, ctrs).
-  Definition repr (x : t) : UContext.t :=
-    let (u, cst) := x in
-    (u, (mapi (fun i _ => Level.lvar i) u, cst)).
-
-  Definition levels (uctx : t) : LevelSet.t :=
-    LevelSetProp.of_list (fst (snd (repr uctx))).
-
-  #[local]
-  Existing Instance EqDec_ReflectEq.
-  Definition inter (au av : AUContext.t) : AUContext.t :=
-    let prefix := (split_prefix au.1 av.1).1.1 in
-    let lvls := fold_left_i (fun s i _ => LevelSet.add (Level.lvar i) s) prefix LevelSet.empty in
-    let filter := ConstraintSet.filter (is_declared_cstr_levels lvls) in
-    make prefix (ConstraintSet.union (filter au.2) (filter av.2)).
-End AUContext.
-
-Module ContextSet.
-  Definition t := LevelSet.t × ConstraintSet.t.
-
-  Definition levels : t -> LevelSet.t := fst.
-  Definition constraints : t -> ConstraintSet.t := snd.
-
-  Definition empty : t := (LevelSet.empty, ConstraintSet.empty).
-
-  Definition is_empty (uctx : t)
-    := LevelSet.is_empty (fst uctx) && ConstraintSet.is_empty (snd uctx).
-
-  Definition Equal (x y : t) : Prop :=
-    x.1 =_lset y.1 /\ x.2 =_cset y.2.
-
-  Definition equal (x y : t) : bool :=
-    x.1 ==_lset y.1 && x.2 ==_cset y.2.
-
-  Definition Subset (x y : t) : Prop :=
-    LevelSet.Subset (levels x) (levels y) /\
-    ConstraintSet.Subset (constraints x) (constraints y).
-
-  Definition subset (x y : t) : bool :=
-    LevelSet.subset (levels x) (levels y) &&
-    ConstraintSet.subset (constraints x) (constraints y).
-
-  Definition inter (x y : t) : t :=
-    (LevelSet.inter (levels x) (levels y),
-      ConstraintSet.inter (constraints x) (constraints y)).
-
-  Definition inter_spec (x y : t) :
-    Subset (inter x y) x /\
-      Subset (inter x y) y /\
-      forall z, Subset z x -> Subset z y -> Subset z (inter x y).
-  Proof.
-    split; last split.
-    1,2: split=> ?; [move=> /LevelSet.inter_spec [//]|move=> /ConstraintSet.inter_spec [//]].
-    move=> ? [??] [??]; split=> ??;
-    [apply/LevelSet.inter_spec|apply/ConstraintSet.inter_spec]; split; auto.
-  Qed.
-
-  Definition union (x y : t) : t :=
-    (LevelSet.union (levels x) (levels y), ConstraintSet.union (constraints x) (constraints y)).
-
-  Definition union_spec (x y : t) :
-    Subset x (union x y) /\
-      Subset y (union x y) /\
-      forall z, Subset x z -> Subset y z -> Subset (union x y) z.
-  Proof.
-    split; last split.
-    1,2: split=> ??; [apply/LevelSet.union_spec|apply/ConstraintSet.union_spec ]; by constructor.
-    move=> ? [??] [??]; split=> ?;
-    [move=>/LevelSet.union_spec|move=>/ConstraintSet.union_spec]=>-[]; auto.
-  Qed.
-
-  Lemma equal_spec s s' : equal s s' <-> Equal s s'.
-  Proof.
-    rewrite /equal/Equal/is_true Bool.andb_true_iff LevelSet.equal_spec ConstraintSet.equal_spec.
-    reflexivity.
-  Qed.
-
-  Lemma subset_spec s s' : subset s s' <-> Subset s s'.
-  Proof.
-    rewrite /subset/Subset/is_true Bool.andb_true_iff LevelSet.subset_spec ConstraintSet.subset_spec.
-    reflexivity.
-  Qed.
-
-  Lemma subsetP s s' : reflect (Subset s s') (subset s s').
-  Proof.
-    generalize (subset_spec s s').
-    destruct subset; case; constructor; intuition.
-  Qed.
-End ContextSet.
-
-Export (hints) ContextSet.
-
-Notation "(=_cs)" := ContextSet.Equal (at level 0).
-Notation "(⊂_cs)" := ContextSet.Subset (at level 0).
-Infix "=_cs" := ContextSet.Equal (at level 30).
-Infix "⊂_cs" := ContextSet.Subset (at level 30).
-Notation "(==_cs)" := ContextSet.equal (at level 0).
-Notation "(⊂?_cs)" := ContextSet.subset (at level 0).
-Infix "==_cs" := ContextSet.equal (at level 30).
-Infix "⊂?_cs" := ContextSet.subset (at level 30).
-
-Lemma incl_cs_refl cs : cs ⊂_cs cs.
-Proof.
-  split; [lsets|csets].
-Qed.
-
-Lemma incl_cs_trans cs1 cs2 cs3 : cs1 ⊂_cs cs2 -> cs2 ⊂_cs cs3 -> cs1 ⊂_cs cs3.
-Proof.
-  intros [? ?] [? ?]; split; [lsets|csets].
-Qed.
-
-Lemma empty_contextset_subset u : ContextSet.empty ⊂_cs u.
-Proof.
-  red. split; cbn; [lsets|csets].
-Qed.
-
-(* Variance info is needed to do full universe polymorphism *)
-Module Variance.
-  (** A universe position in the instance given to a cumulative
-     inductive can be the following. Note there is no Contralvariant
-     case because [forall x : A, B <= forall x : A', B'] requires [A =
-     A'] as opposed to [A' <= A]. *)
-  Inductive t :=
-  | Irrelevant : t
-  | Covariant : t
-  | Invariant : t.
-  Derive NoConfusion EqDec for t.
-
-  (* val check_subtype : t -> t -> bool *)
-  (* val sup : t -> t -> t *)
-End Variance.
-
-(** What to check of two instances *)
-Variant opt_variance :=
-  AllEqual | AllIrrelevant | Variance of list Variance.t.
-
-Inductive universes_decl : Type :=
-| Monomorphic_ctx
-| Polymorphic_ctx (cst : AUContext.t).
-
-Derive NoConfusion for universes_decl.
-
-Definition levels_of_udecl u :=
-  match u with
-  | Monomorphic_ctx => LevelSet.empty
-  | Polymorphic_ctx ctx => AUContext.levels ctx
-  end.
-
-Definition constraints_of_udecl u :=
-  match u with
-  | Monomorphic_ctx => ConstraintSet.empty
-  | Polymorphic_ctx ctx => snd (snd (AUContext.repr ctx))
-  end.
-
-Declare Scope univ_scope.
-Delimit Scope univ_scope with u.
-
-Inductive satisfies0 (v : valuation) : UnivConstraint.t -> Prop :=
-| satisfies0_Lt (l l' : Level.t) (z : Z) : (Z.of_nat (val v l) <= Z.of_nat (val v l') - z)%Z
-                        -> satisfies0 v (l, ConstraintType.Le z, l')
-| satisfies0_Eq (l l' : Level.t) : val v l = val v l'
-                        -> satisfies0 v (l, ConstraintType.Eq, l').
-
-Definition satisfies v : ConstraintSet.t -> Prop :=
-  ConstraintSet.For_all (satisfies0 v).
-
-Lemma satisfies_union v φ1 φ2 :
-  satisfies v (CS.union φ1 φ2)
-  <-> (satisfies v φ1 /\ satisfies v φ2).
-Proof using Type.
-  unfold satisfies. split.
-  - intros H; split; intros c Hc; apply H; now apply CS.union_spec.
-  - intros [H1 H2] c Hc; apply CS.union_spec in Hc; destruct Hc; auto.
-Qed.
-
-Lemma satisfies_subset φ φ' val :
-  ConstraintSet.Subset φ φ' ->
-  satisfies val φ' ->
-  satisfies val φ.
-Proof using Type.
-  intros sub sat ? isin.
-  apply sat, sub; auto.
-Qed.
-
-Definition consistent ctrs := exists v, satisfies v ctrs.
-
-Definition consistent_extension_on cs cstr :=
-  forall v, satisfies v (ContextSet.constraints cs) -> exists v',
-      satisfies v' cstr /\
-        LevelSet.For_all (fun l => val v l = val v' l) (ContextSet.levels cs).
-
-Lemma consistent_extension_on_empty Σ :
-  consistent_extension_on Σ CS.empty.
-Proof using Type.
-  move=> v hv; exists v; split; [move=> ? /CS.empty_spec[]| move=> ??//].
-Qed.
-
-Lemma consistent_extension_on_union X cstrs
-  (wfX : forall c, CS.In c X.2 -> LS.In c.1.1 X.1 /\ LS.In c.2 X.1) :
-  consistent_extension_on X cstrs <->
-  consistent_extension_on X (CS.union cstrs X.2).
-Proof using Type.
-  split.
-  2: move=> h v /h [v' [/satisfies_union [??] eqv']]; exists v'; split=> //.
-  move=> hext v /[dup] vsat /hext [v' [v'sat v'eq]].
-  exists v'; split=> //.
-  apply/satisfies_union; split=> //.
-  move=> c hc. destruct (wfX c hc).
-  destruct (vsat c hc); constructor; rewrite -!v'eq //.
-Qed.
-
-
-Definition leq0_universe_n n φ (u u' : Universe.t) :=
-  forall v, satisfies v φ -> (Z.of_nat (val v u) <= Z.of_nat (val v u') - n)%Z.
-
-Definition leq_universe_n {cf} n φ (u u' : Universe.t) :=
-  if check_univs then leq0_universe_n n φ u u' else True.
-
-Definition lt_universe {cf} := leq_universe_n 1.
-Definition leq_universe {cf} := leq_universe_n 0.
-
-Definition eq0_universe φ (u u' : Universe.t) :=
-  forall v, satisfies v φ -> val v u = val v u'.
-
-Definition eq_universe {cf} φ (u u' : Universe.t) :=
-  if check_univs then eq0_universe φ u u' else True.
-
-(* ctrs are "enforced" by φ *)
-
-Definition valid_constraints0 φ ctrs
-  := forall v, satisfies v φ -> satisfies v ctrs.
-
-Definition valid_constraints {cf} φ ctrs
-  := if check_univs then valid_constraints0 φ ctrs else True.
-
-Definition compare_universe {cf} φ (pb : conv_pb) :=
-  match pb with
-  | Conv => eq_universe φ
-  | Cumul => leq_universe φ
-  end.
-
-
-Ltac unfold_univ_rel0 :=
-  unfold eq0_universe, leq0_universe_n, valid_constraints0 in *;
-  try (
-    match goal with |- forall v : valuation, _ -> _ => idtac end;
-    intros v Hv;
-    repeat match goal with H : forall v : valuation, _ -> _ |- _ => specialize (H v Hv) end;
-    cbnr
-  ).
-
-Ltac unfold_univ_rel :=
-  unfold eq_universe, leq_universe, lt_universe, leq_universe_n, valid_constraints in *;
-  destruct check_univs; [unfold_univ_rel0 | trivial].
-
-Section Univ.
-  Context {cf}.
-
-  Lemma valid_subset φ φ' ctrs
-    : ConstraintSet.Subset φ φ' -> valid_constraints φ ctrs
-      ->  valid_constraints φ' ctrs.
-  Proof using Type.
-    unfold_univ_rel.
-    intros Hφ H v Hv. apply H.
-    intros ctr Hc. apply Hv. now apply Hφ.
-  Qed.
-
-  Lemma switch_minus (x y z : Z) : (x <= y - z <-> x + z <= y)%Z.
-  Proof using Type. split; lia. Qed.
-
-  (** **** Lemmas about eq and leq **** *)
-
-  Global Instance eq_universe_refl φ : Reflexive (eq_universe φ).
-  Proof using Type.
-    intros u; unfold_univ_rel.
-  Qed.
-
-  Global Instance leq_universe_refl φ : Reflexive (leq_universe φ).
-  Proof using Type.
-    intros u; unfold_univ_rel. lia.
-  Qed.
-
-  Global Instance eq_universe_sym φ : Symmetric (eq_universe φ).
-  Proof using Type.
-    intros u u' H; unfold_univ_rel.
-    lia.
-  Qed.
-
-  Global Instance eq_universe_trans φ : Transitive (eq_universe φ).
-  Proof using Type.
-    intros u u' u'' H1 H2; unfold_univ_rel.
-    lia.
-  Qed.
-
-  Global Instance leq_universe_n_trans n φ : Transitive (leq_universe_n (Z.of_nat n) φ).
-  Proof using Type.
-    intros u u' u'' H1 H2; unfold_univ_rel.
-    lia.
-  Qed.
-
-  Global Instance leq_universe_trans φ : Transitive (leq_universe φ).
-  Proof using Type. apply (leq_universe_n_trans 0). Qed.
-
-  Global Instance lt_universe_trans φ : Transitive (lt_universe φ).
-  Proof using Type. apply (leq_universe_n_trans 1). Qed.
-
-  Lemma eq0_leq0_universe φ u u' :
-    eq0_universe φ u u' <-> leq0_universe_n 0 φ u u' /\ leq0_universe_n 0 φ u' u.
-  Proof using Type.
-    split.
-    - intros H. split; unfold_univ_rel0; lia.
-    - intros [H1 H2]. unfold_univ_rel0; lia.
-  Qed.
-
-  Lemma eq_universe_leq_universe φ u u' :
-    eq_universe φ u u' <-> leq_universe φ u u' /\ leq_universe φ u' u.
-  Proof using Type.
-    unfold_univ_rel => //.
-    apply eq0_leq0_universe.
-  Qed.
-
-  Lemma leq_universe_sup_l φ u1 u2 : leq_universe φ u1 (Universe.sup u1 u2).
-  Proof using Type. unfold_univ_rel. rewrite val_sup; lia. Qed.
-
-  Lemma leq_universe_sup_r φ u1 u2 : leq_universe φ u2 (Universe.sup u1 u2).
-  Proof using Type. unfold_univ_rel. rewrite val_sup; lia. Qed.
-
-  Lemma leq_universe_sup_mon φ u1 u1' u2 u2' : leq_universe φ u1 u1' -> leq_universe φ u2 u2' ->
-    leq_universe φ (Universe.sup u1 u2) (Universe.sup u1' u2').
-  Proof using Type.
-    intros H1 H2; unfold_univ_rel.
-    rewrite !val_sup. lia.
-  Qed.
-
-  Global Instance eq_leq_universe φ : subrelation (eq_universe φ) (leq_universe φ).
-  Proof using Type.
-    intros u u'. apply eq_universe_leq_universe.
-  Qed.
-
-  Global Instance eq_universe_equivalence φ : Equivalence (eq_universe φ) := Build_Equivalence _ _ _ _.
-
-  Global Instance leq_universe_preorder φ : PreOrder (leq_universe φ) := Build_PreOrder _ _ _.
-
-  Global Instance lt_universe_irrefl {c: check_univs} φ (H: consistent φ) : Irreflexive (lt_universe φ).
-  Proof using Type.
-    intro u. unfold complement.
-    unfold_univ_rel => //.
-    destruct H as [v Hv]; intros nH; specialize (nH v Hv); lia.
-  Qed.
-
-  Global Instance lt_universe_str_order {c: check_univs} φ (H: consistent φ) : StrictOrder (lt_universe φ).
-  Proof.
-    refine (Build_StrictOrder _ _ _).
-    now unshelve eapply lt_universe_irrefl.
-  Qed.
-
-  Global Instance leq_universe_antisym φ : Antisymmetric _ (eq_universe φ) (leq_universe φ).
-  Proof using Type. intros t u tu ut. now apply eq_universe_leq_universe. Qed.
-
-  Global Instance leq_universe_partial_order φ
-    : PartialOrder (eq_universe φ) (leq_universe φ).
-  Proof.
-    intros x y; split; apply eq_universe_leq_universe.
-  Defined.
-
-
-  Global Instance compare_universe_subrel φ pb : subrelation (eq_universe φ) (compare_universe φ pb).
-  Proof using Type.
-    destruct pb; tc.
-  Qed.
-
-  Global Instance compare_universe_refl φ pb : Reflexive (compare_universe φ pb).
-  Proof using Type.
-    destruct pb; tc.
-  Qed.
-
-  Global Instance compare_universe_trans φ pb : Transitive (compare_universe φ pb).
-  Proof using Type.
-    destruct pb; tc.
-  Qed.
-
-  Global Instance compare_universe_preorder φ pb : PreOrder (compare_universe φ pb).
-  Proof using Type.
-    destruct pb; tc.
-  Qed.
-
-  Definition eq_leq_universe' φ u u'
-    := @eq_leq_universe φ u u'.
-  Definition leq_universe_refl' φ u
-    := @leq_universe_refl φ u.
-
-  Hint Resolve eq_leq_universe' leq_universe_refl' : core.
-
-
-  Lemma cmp_universe_subset φ φ' pb t u :
-    ConstraintSet.Subset φ φ' -> compare_universe φ pb t u -> compare_universe φ' pb t u.
-  Proof using Type.
-    intros Hctrs.
-    destruct pb, t, u; cbnr; trivial.
-    all: intros H; unfold_univ_rel;
-    apply H.
-    all: eapply satisfies_subset; eauto.
-  Qed.
-
-  Lemma eq_universe_subset φ φ' t u
-    : ConstraintSet.Subset φ φ'
-      -> eq_universe φ t u -> eq_universe φ' t u.
-  Proof using Type. apply cmp_universe_subset with (pb := Conv). Qed.
-
-  Lemma leq_universe_subset φ φ' t u
-    : ConstraintSet.Subset φ φ'
-      -> leq_universe φ t u -> leq_universe φ' t u.
-  Proof using Type. apply cmp_universe_subset with (pb := Cumul). Qed.
-
-End Univ.
-
-Module Sort.
-  Inductive t_ {univ} :=
-    sProp | sSProp | sType (_ : univ).
-  Derive NoConfusion for t_.
-  Arguments t_ : clear implicits.
-
-  Definition t := t_ Universe.t.
-
-  Inductive family : Set :=
-  | fSProp
-  | fProp
-  | fType.
-  Derive NoConfusion EqDec for family.
-
-  Definition eqb {univ} `{ReflectEq univ} (u1 u2 : t_ univ) : bool :=
-    match u1, u2 with
-    | sSProp, sSProp => true
-    | sProp, sProp => true
-    | sType e1, sType e2 => eqb e1 e2
-    | _, _ => false
-    end.
-
-  #[global, program] Instance reflect_eq_sort {univ} `{ReflectEq univ} : ReflectEq (t_ univ) :=
-    { eqb := eqb }.
-  Next Obligation.
-    destruct x, y; cbn; try constructor; auto; try congruence.
-    destruct (eqb_spec u u0); constructor. now f_equal.
-    congruence.
-  Qed.
-
-  #[global] Instance eq_dec_sort {univ} `{EqDec univ} : EqDec (t_ univ) := ltac:(intros s s'; decide equality).
-
-  Definition map {u u'} (f : u -> u') s :=
-    match s with
-    | sType u => sType (f u)
-    | sProp => sProp
-    | sSProp => sSProp
-    end.
-
-  Definition on_sort {univ} {T} (P: univ -> T) (def: T) (s : t_ univ) :=
-    match s with
-    | sProp | sSProp => def
-    | sType l => P l
-    end.
-
-  (** Test if the universe is a lub of levels or contains +n's. *)
-  Definition is_levels (s : t) : bool :=
-    match s with
+    match u.(s) with
     | sSProp | sProp => true
-    | sType l => Universe.is_levels l
+    | sType => UnivLvl.is_level u.(l)
     end.
 
-  (** Test if the universe is a level or an algebraic universe. *)
-  Definition is_level (s : t) : bool :=
-    match s with
-    | sSProp | sProp => true
-    | sType l => Universe.is_level l
-    end.
-
-  Definition is_sprop {univ} (s : t_ univ) : bool :=
-    match s with
+  Definition is_sprop {ulvl} (u : t_ Sort.t ulvl) : bool :=
+    match u.(s) with
       | sSProp => true
       | _ => false
     end.
 
-  Definition is_prop {univ} (s : t_ univ) : bool :=
-    match s with
+  Definition is_prop {ulvl} (u : t_ Sort.t ulvl) : bool :=
+    match u.(s) with
       | sProp => true
       | _ => false
     end.
 
-  Definition is_propositional {univ} (s : t_ univ) : bool :=
-    match s with
+  Definition is_propositional {ulvl} (u : t_ Sort.t ulvl) : bool :=
+    match u.(s) with
       | sProp | sSProp => true
       | _ => false
     end.
 
-  Lemma is_prop_propositional {univ} (s : t_ univ) :
-    is_prop s -> is_propositional s.
-  Proof. now destruct s. Qed.
-  Lemma is_sprop_propositional {univ} (s : t_ univ) :
-    is_sprop s -> is_propositional s.
-  Proof. now destruct s. Qed.
+  Lemma is_prop_propositional {ulvl} (u : t_ Sort.t ulvl) :
+    is_prop u -> is_propositional u.
+  Proof. destruct u as [s l]; now destruct s. Qed.
+  Lemma is_sprop_propositional {ulvl} (u : t_ Sort.t ulvl) :
+    is_sprop u -> is_propositional u.
+  Proof. destruct u as [s l]; now destruct s. Qed.
 
-  Definition is_type_sort {univ} (s : t_ univ) : bool :=
-    match s with
-      | sType _ => true
+  Definition is_type_sort {ulvl} (u : t_ Sort.t ulvl) : bool :=
+    match u.(s) with
+      | sType => true
       | _ => false
     end.
 
-  Definition type0 : t := sType (Universe.make LevelExpr.set).
-  Definition type1 : t := sType (Universe.make LevelExpr.type1).
+  Definition type0 : t := mkUniv sType UnivLvl.type0.
+  Definition type1 : t := mkUniv sType UnivLvl.type1.
 
   Definition of_levels (l : PropLevel.t + Level.t) : t :=
     match l with
-    | inl PropLevel.lSProp => sSProp
-    | inl PropLevel.lProp => sProp
-    | inr l => sType (Universe.make' l)
+    | inl PropLevel.lSProp => mkUniv sSProp UnivLvl.type0
+    | inl PropLevel.lProp => mkUniv sProp UnivLvl.type0
+    | inr l => mkUniv sType (UnivLvl.make' l)
     end.
 
   (** The universe strictly above FOR TYPING (not cumulativity) *)
 
-  Definition super_ {univ} type1 univ_succ (s : t_ univ) : t_ univ :=
-    match s with
-    | sSProp | sProp => sType type1
-    | sType l => sType (univ_succ l)
+  Definition super_ {ulvl} type1 usucc (u : t_ Sort.t ulvl) : t_ Sort.t ulvl :=
+    match u.(s) with
+    | sSProp | sProp => mkUniv sType type1
+    | sType => mkUniv sType (usucc u.(l))
     end.
-  Definition super : t -> t := super_ (Universe.make LevelExpr.type1) Universe.succ.
+  Definition super : t -> t := super_ UnivLvl.type1 UnivLvl.succ.
   Definition csuper := super_ 1 S.
 
-  Definition sup_ {univ} univ_sup (s s' : t_ univ) : t_ univ :=
-    match s, s' with
-    | sSProp, s' => s'
-    | sProp, sSProp => sProp
-    | sProp, s' => s'
-    | sType u1, sType u2 => sType (univ_sup u1 u2)
-    | sType _ as s, _ => s
+  Definition sup_ {ulvl} type0 univ_sup (u u' : t_ Sort.t ulvl) : t_ Sort.t ulvl :=
+    match u.(s), u'.(s) with
+    | sSProp, _ => u'
+    | sProp, sSProp => mkUniv sProp type0
+    | sProp, _ => u'
+    | sType, sType => mkUniv sType (univ_sup u.(l) u'.(l))
+    | sType, _ => u
     end.
-  Definition sup : t -> t -> t := sup_ Universe.sup.
-  Definition csup := sup_ Nat.max.
+  Definition sup : t -> t -> t := sup_ UnivLvl.type0 UnivLvl.sup.
+  Definition csup := sup_ 0 Nat.max.
 
   (** Type of a product *)
-  Definition sort_of_product_ {univ} univ_sup (domsort rangsort : t_ univ) : t_ univ :=
-    match rangsort with
-    | sSProp | sProp => rangsort
+  Definition sort_of_product_ {ulvl} type0 usup (dom codom : t_ Sort.t ulvl) : t_ Sort.t ulvl :=
+    match codom.(s) with
+    | sSProp | sProp => codom
     (* Prop and SProp impredicativity *)
-    | _ => Sort.sup_ univ_sup domsort rangsort
+    | _ => sup_ type0 usup dom codom
     end.
-  Definition sort_of_product : t -> t -> t := sort_of_product_ Universe.sup.
-  Definition csort_of_product := sort_of_product_ Nat.max.
+  Definition sort_of_product : t -> t -> t := sort_of_product_ UnivLvl.type0 UnivLvl.sup.
+  Definition csort_of_product := sort_of_product_ 0 Nat.max.
 
-  Definition get_is_level (s : t) : option Level.t :=
-    match s with
+  Definition get_is_level (u : t) : option Level.t :=
+    match u.(s) with
     | sSProp => None
     | sProp => None
-    | sType l => Universe.get_is_level l
+    | sType => UnivLvl.get_is_level u.(l)
     end.
 
-  Definition to_family {univ} (s : t_ univ) :=
-    match s with
-    | sSProp => fSProp
-    | sProp => fProp
-    | sType _ => fType
+  Definition to_family {sort ulvl} (u : t_ sort ulvl) := u.(s).
+
+  Definition to_csort v u :=
+    match u.(s) with
+    | sSProp => mkUniv sSProp 0
+    | sProp => mkUniv sProp 0
+    | sType => mkUniv sType (val v u.(l))
     end.
 
-  Definition to_csort v s :=
-    match s with
-    | sSProp => sSProp
-    | sProp => sProp
-    | sType u => sType (val v u)
-    end.
-
-  Lemma to_family_to_csort s v :
-    to_family (to_csort v s) = to_family s.
+  Lemma to_family_to_csort u v :
+    to_family (to_csort v u) = to_family u.
   Proof.
-    destruct s; cbnr.
+    destruct u as [s l]; unfold to_csort; destruct s; cbnr.
   Qed.
 
-  Lemma sType_super_ {univ type1 univ_succ} (s : t_ univ) :
-    to_family (super_ type1 univ_succ s) = fType.
-  Proof. now destruct s. Qed.
+  Lemma sType_super_ {ulvl type1 usucc} (u : t_ Sort.t ulvl) :
+    to_family (super_ type1 usucc u) = sType.
+  Proof. destruct u as [s l]; now destruct s. Qed.
 
   Lemma sType_super (s : t) :
-    to_family (super s) = fType.
+    to_family (super s) = sType.
   Proof. apply sType_super_. Qed.
 
-  Inductive lt_ {univ univ_lt} : t_ univ -> t_ univ -> Prop :=
-  | ltPropSProp : lt_ sProp sSProp
-  | ltPropType s : lt_ sProp (sType s)
-  | ltSPropType s : lt_ sSProp (sType s)
-  | ltTypeType s1 s2 : univ_lt s1 s2 -> lt_ (sType s1) (sType s2).
+  (* XXX: should only be used for MSetAVL so it should be fine to simply give the lexicographical order? *)
+  Inductive lt_ {ulvl ult} : t_ Sort.t ulvl -> t_ Sort.t ulvl -> Prop :=
+  | ltPropSProp i : lt_ (mkUniv sProp i) (mkUniv sSProp i)
+  | ltPropType i l :  lt_ (mkUniv sProp i) (mkUniv sType l)
+  | ltSPropType i l : lt_ (mkUniv sSProp i) (mkUniv sType l)
+  | ltTypeType l1 l2 : ult l1 l2 -> lt_ (mkUniv sType l1) (mkUniv sType l2).
   Derive Signature for lt_.
-  Arguments lt_ {univ} univ_lt.
+  Arguments lt_ {ulvl} ult.
 
-  Definition lt := lt_ Universe.lt.
+  Definition lt := lt_ UnivLvl.lt.
   Definition clt := lt_ Nat.lt.
 
   Module OT <: OrderedType.
@@ -1639,9 +189,9 @@ Module Sort.
     #[local] Instance lt_strorder : StrictOrder lt.
     Proof.
       constructor.
-      - intros [| |] X; inversion X.
-        now eapply irreflexivity in H1.
-      - intros [| |] [| |] [| |] X1 X2;
+      - intros [ [| |] u ] X; inversion X.
+	    now eapply irreflexivity in H1.
+      - intros [ [| |] u ] [ [| |] v ] [ [| |] w ] X1 X2;
           inversion X1; inversion X2; constructor.
         subst.
         etransitivity; tea.
@@ -1651,39 +201,46 @@ Module Sort.
     Proof.
       intros x y e z t e'. hnf in * |- ; subst. reflexivity.
     Qed.
-    Definition compare (x y : t) : comparison
-      := match x, y with
+	
+    Definition compare (u v : t) : comparison
+      := match u.(s), v.(s) with
           | sProp, sProp => Eq
           | sProp, _ => Lt
           | _, sProp => Gt
           | sSProp, sSProp => Eq
           | sSProp, _ => Lt
           | _, sSProp => Gt
-          | sType x, sType y => LevelExprSet.compare x y
+          | sType, sType => LevelExprSet.compare u.(l) v.(l)
           end.
+
     Lemma compare_spec x y : CompareSpec (eq x y) (lt x y) (lt y x) (compare x y).
     Proof.
       cbv [compare eq].
-      destruct x, y.
+
+      destruct x as [ [| |] l ]; destruct y as [ [| |] l' ]; cbn.
       all: lazymatch goal with
             | [ |- context[LevelExprSet.compare ?x ?y] ]
               => destruct (LevelExprSet.compare_spec x y)
             | _ => idtac
             end.
+
       all: lazymatch goal with
             | [ H : LevelExprSet.eq (?f ?x) (?f ?y) |- _ ]
               => apply LevelExprSet.eq_leibniz in H;
-                is_var x; is_var y; destruct x, y; cbn in H; subst
+                is_var l; is_var l'; destruct x, y; cbn in H; subst
             | _ => idtac
             end.
+
       all: repeat constructor; try apply f_equal; try assumption.
+
+	  
       f_equal; apply Eqdep_dec.UIP_dec; decide equality.
     Qed.
     Definition eq_dec (x y : t) : {x = y} + {x <> y}.
     Proof. repeat decide equality. apply Universe.eq_dec_univ0. Defined.
   End OT.
   Module OTOrig <: OrderedTypeOrig := Backport_OT OT.
-End Sort.
+End Universe.
 
 
 Module SortMap := FMapAVL.Make Sort.OTOrig.
