common/theories/Sorts.v
@@ -1,0 +1,19 @@
+From Stdlib Require Import OrdersAlt MSetList MSetAVL MSetFacts MSetProperties MSetDecide FMapAVL.
+From Equations Require Import Equations.
+From MetaRocq.Utils Require Import utils MRMSets MRFSets.
+From MetaRocq.Common Require Import BasicAst config Levels.
+From Stdlib Require Import ssreflect.
+
+Local Open Scope nat_scope.
+Local Open Scope string_scope2.
+
+Implicit Types (cf : checker_flags).
+
+Module Sort.
+  Variant t := sProp | sSProp | sType.
+  Derive NoConfusion EqDec for t.
+End Sort.
+
+Notation sProp := Sort.sProp.
+Notation sSProp := Sort.sSProp.
+Notation sType := Sort.sType.
